Switch to separation logic over memory
Unify ghost state and memory into a single memory from variables to
arbitrarily-typed values (distinguishing between ghost and regular
variables). Variables are now dynamic, with a primitive to allocate
them. Specs will use separation logic over memory variables, with
assertions capturing that uses of variables to Gets and Assgns are
well-typed (Get returns a value of the expected type, failing otherwise;
the precondition guarantees this doesn't happen, and Assgns are similar,
guaranteeing the type of a variable doesn't change).

src/CCLHoareTriples.v
@@ -4,15 +4,14 @@ Import CCLTactics.
 
 Section HoareTriples.
 
-  Context {St:StateTypes}.
-  Variables G:Protocol St.
+  Variables G:Protocol.
 
   Record SpecParams T :=
     { precondition :  Prop;
-      postcondition : (Sigma St * Sigma St) ->
+      postcondition : (Sigma * Sigma) ->
                       T -> Prop }.
 
-  Definition Spec A T := A -> (Sigma St * Sigma St) -> SpecParams T.
+  Definition Spec A T := A -> (Sigma * Sigma) -> SpecParams T.
 
   Definition cprog_spec tid A T' (spec: Spec A T') (p: cprog T') :=
     forall T (rx: _ -> cprog T),
@@ -40,16 +39,16 @@ Section HoareTriples.
   correctness statement - [cprog_spec] instead unquotes triple into a double
   (with an arbitrary continuation) and then uses the double-based correctness
   statement *)
-  Definition cprog_triple A T tid (spec: Spec A T) (p: @cprog St T) :=
+  Definition cprog_triple A T tid (spec: Spec A T) (p: cprog T) :=
     forall a st out,
       precondition (spec a st) ->
       exec G tid st p out ->
       match out with
-      | Finished sigma_i' sigma' v => postcondition (spec a st) (sigma_i', sigma') v
+      | Finished st' v => postcondition (spec a st) st' v
       | Error => False
       end.
 
-  Theorem triple_spec_equiv : forall A T tid (spec: Spec A T) (p: @cprog St T),
+  Theorem triple_spec_equiv : forall A T tid (spec: Spec A T) (p: cprog T),
       cprog_spec tid spec p <->
       cprog_triple tid spec p.
   Proof.
@@ -90,8 +89,8 @@ Section HoareTriples.
       exec G tid st p out ->
       precondition (spec a st) ->
       match out with
-        | Finished sigma_i' sigma' v =>
-          postcondition (spec a st) (sigma_i', sigma') v
+        | Finished st' v =>
+          postcondition (spec a st) st' v
         | Error => False
       end.
   Proof.
