src/Automation.v
@@ -42,3 +42,31 @@ Ltac inj_pair2 :=
   | [ H: existT ?P ?a _ = existT ?P ?a _ |- _ ] =>
     apply inj_pair2 in H; subst
   end.
+
+(* BUG: Coq doesn't accept this, complaining that n is not in scope, but it
+works perfectly well within a proof script (and correctly bind n,m to the names
+used in the pattern match) *)
+(* Ltac break_tuple :=
+  repeat match goal with
+         | [ H: context[let '(n, m) := ?a in _] |- _ ] =>
+           let n := fresh n in
+           let m := fresh m in
+           destruct a as [n m]
+         end. *)
+
+Inductive Learnt {P:Prop} :=
+| AlreadyLearnt (H:P).
+
+Ltac learn_fact H :=
+  let P := type of H in
+  let P := eval simpl in P in
+  lazymatch goal with
+    (* matching the type of H with the Learnt hypotheses means the
+    learning fails even when the proposition is known by a different
+    but unifiable type term *)
+  | [ Hlearnt: @Learnt P |- _ ] =>
+    fail 0 "already knew" P "through" Hlearnt
+  | _ => pose proof (H:P); pose proof (@AlreadyLearnt P H)
+  end.
+
+Tactic Notation "learn" "that" constr(H) := learn_fact H.
